<http://ontolog.cim3.net/file/work/OntologySummit2013/Hackathon-Clinics/HC-05_Ontology-of-OntologyEvaluation/owl/ontology>
  a owl:Ontology;
  owl:versionInfo "$Id$".

@prefix : <http://ontolog.cim3.net/ontology/evaluation#> .

:Ontology
  a owl:Class;
  rdfs:comment "An ontology is a living artifact that is born inside an organizational context, has a life-cycle and is interacted with by various agents.  Examples of ontologies are the Gene Ontology or OWL Time, which may have multiple representations and/or versions.";
  rdfs:subClassOf
    [ a owl:Restriction;
      owl:onProperty :manifestedBy;
      owl:allValuesFrom :OntologyRepresentation ],
    [ a owl:Restriction;
      owl:onProperty :hasCharacteristic;
      owl:minCardinality 0 ].

:OntologyRepresentation
  a owl:Class;
  rdfs:subClassOf
    [ a owl:Restriction;
      owl:onProperty :hasCharacteristic;
      owl:minCardinality 0 ].

:FormalOntology
  a owl:Class.

:ConceptualOntologyRepresentation
  a owl:Class;
  rdfs:label "ontology (conceptual model)";
  rdfs:comment "A human-centric, human-understandable model of the things and relationships in a portion of the world, expressed independently of technological implementation or machine use considerations. May be textual, graphical, or captured in any other human-friendly way.";
  rdfs:subClassOf :OntologyRepresentation.

:LogicalOntologyRepresentation
  a owl:Class;
  rdfs:label "ontology (logical model)";
  rdfs:comment "A representation of an ontology in a particular, logic-based ontology language, such as OWL 2, Common Logic, etc.";
  rdfs:subClassOf :OntologyRepresentation, :FormalOntology.

:PhysicalOntologyRepresentation
  a owl:Class;
  rdfs:label "ontology (physical model)";
  rdfs:comment "A serialized representation of an LogicalOntologyRepresentation (e.g., in RDF/XML or CLIF)";
  rdfs:subClassOf :OntologyRepresentation, :FormalOntology.

:hasCharacteristic
  a owl:ObjectProperty.

# definition that should have been included from High Level Concept Model

:OntologyLanguage
  a owl:Class;
  rdfs:comment "Language used to represent an ontology, e.g. OWL, Common Logic, etc. An ontology characteristic.".

# suggested additional definitions

:OWL2 a :OntologyLanguage.
:CommonLogic a :OntologyLanguage.
:RDFS a :OntologyLanguage;
  rdfs:label "RDF Schema".

:LogicalOntologyRepresentation
  rdfs:subClassOf
    [ a owl:Restriction;
      owl:onProperty :implements;
      owl:allValuesFrom :ConceptualOntologyRepresentation ].

:PhysicalOntologyRepresentation
  rdfs:subClassOf
    [ a owl:Restriction;
      owl:onProperty :implements;
      owl:allValuesFrom :LogicalOntologyRepresentation ].

:OntologySerializationFormat
  a owl:Class;
  rdfs:comment "Format used to serialize a physical ontology, e.g. RDF/XML or CLIF. An ontology characteristic.".

:RDF_XML a :OntologySerializationFormat.

:OWL_XML a :OntologySerializationFormat.

:Turtle a :OntologySerializationFormat;
  rdfs:comment "Terse RDF Triple Language".
    
:CLIF a :OntologySerializationFormat;
  rdfs:comment "Common Logic Interchange Format".

:XCL a :OntologySerializationFormat;
  rdfs:comment "XML representation for Common Logic".

# TODO:  reflect :OntologyLanguage as :hasCharacteristic of :LogicalOntologyRepresentation

# TODO:  reflect :OntologySerializationFormat as :hasCharacteristic of :PhysicalOntologyRepresentation

# TODO:  link ontology serialization formats to their respective ontology languages?
